theories/std/for_.v
@@ -1,0 +1,396 @@
+From heap_lang Require Import
+  prelude.
+From heap_lang.language Require Import
+  notations
+  proofmode.
+From heap_lang.std Require Export
+  base.
+
+Section heap_GS.
+  Context `{heap_GS : !heapGS Σ}.
+
+  Implicit Types δ : nat.
+  Implicit Types fn : val.
+
+  Definition for_ : val :=
+    rec: "for" "beg" "end" "fn" :=
+      if: "end" ≤ "beg" then (
+        #()
+      ) else (
+        "fn" "beg" ;;
+        "for" (#1 + "beg") "end" "fn"
+      ).
+
+  #[local] Lemma for_spec_stronger beg i δ Ψ _end fn :
+    i = (beg + δ)%Z →
+    {{{
+      ▷ Ψ i δ ∗
+      □ (
+        ∀ i δ,
+        ⌜i = (beg + δ)%Z ∧ (i < _end)%Z⌝ -∗
+        Ψ i δ -∗
+        WP fn #i {{ res,
+          ⌜res = #()⌝ ∗
+          ▷ Ψ (1 + i)%Z (S δ)
+        }}
+      )
+    }}}
+      for_ #i #_end fn
+    {{{
+      RET #();
+      Ψ (i `max` _end)%Z (δ + Z.to_nat (_end - i))
+    }}}.
+  Proof.
+    iIntros "%Hi %Φ (HΨ & #Hfn) HΦ".
+    remember (Z.to_nat (_end - i)) as ϵ eqn:Hϵ.
+    iInduction ϵ as [| ϵ] "IH" forall (i δ Hi Hϵ);
+      wp_rec; wp_pure credit:"H£"; wp_pures.
+    - assert (i `max` _end = i)%Z as -> by lia. rewrite Nat.add_0_r. iSmash.
+    - rewrite bool_decide_eq_false_2; last lia. wp_pures.
+      wp_apply (wp_wand with "(Hfn [] HΨ)"); first iSmash. iIntros "%res (-> & HΨ)".
+      iMod (lc_fupd_elim_later with "H£ HΨ") as "HΨ".
+      wp_smart_apply ("IH" with "[] [] HΨ [HΦ]"); [iSmash.. |].
+      assert ((1 + i) `max` _end = i `max` _end)%Z as -> by lia. rewrite -Nat.add_succ_comm //.
+  Qed.
+  Lemma for_spec_strong Ψ beg _end fn :
+    {{{
+      ▷ Ψ beg 0 ∗
+      □ (
+        ∀ i δ,
+        ⌜i = (beg + δ)%Z ∧ (i < _end)%Z⌝ -∗
+        Ψ i δ -∗
+        WP fn #i {{ res,
+          ⌜res = #()⌝ ∗
+          ▷ Ψ (1 + i)%Z (S δ)
+        }}
+      )
+    }}}
+      for_ #beg #_end fn
+    {{{
+      RET #();
+      Ψ (beg `max` _end)%Z (Z.to_nat (_end - beg))
+    }}}.
+  Proof.
+    iIntros "%Φ (HΨ & #Hfn) HΦ".
+    wp_apply (for_spec_stronger beg beg 0 with "[$HΨ $Hfn]"); first lia.
+    iSmash.
+  Qed.
+  Lemma for_spec Ψ beg _end fn :
+    (beg ≤ _end)%Z →
+    {{{
+      ▷ Ψ beg 0 ∗
+      □ (
+        ∀ i δ,
+        ⌜i = (beg + δ)%Z ∧ (i < _end)%Z⌝ -∗
+        Ψ i δ -∗
+        WP fn #i {{ res,
+          ⌜res = #()⌝ ∗
+          ▷ Ψ (1 + i)%Z (S δ)
+        }}
+      )
+    }}}
+      for_ #beg #_end fn
+    {{{
+      RET #();
+      Ψ _end (Z.to_nat (_end - beg))
+    }}}.
+  Proof.
+    iIntros "% %Φ H HΦ".
+    wp_apply (for_spec_strong Ψ with "H").
+    rewrite Z.max_r //.
+  Qed.
+  Lemma for_spec_strong' Ψ beg _end fn :
+    {{{
+      ▷ Ψ beg 0 ∗
+      ( [∗ list] δ ∈ seq 0 (Z.to_nat (_end - beg)),
+        ∀ i,
+        ⌜i = (beg + δ)%Z⌝ -∗
+        Ψ i δ -∗
+        WP fn #i {{ res,
+          ⌜res = #()⌝ ∗
+          ▷ Ψ (1 + i)%Z (S δ)
+        }}
+      )
+    }}}
+      for_ #beg #_end fn
+    {{{
+      RET #();
+      Ψ (beg `max` _end)%Z (Z.to_nat (_end - beg))
+    }}}.
+  Proof.
+    iIntros "%Φ (HΨ & Hfn) HΦ".
+    match goal with |- context [big_opL bi_sep (λ _, ?Ξ') _] => set Ξ := Ξ' end.
+    pose (Ψ' i δ := (
+      Ψ i δ ∗
+      [∗ list] ϵ ∈ seq δ (Z.to_nat (_end - beg) - δ), Ξ ϵ
+    )%I).
+    wp_apply (for_spec_strong Ψ' with "[HΨ Hfn]"); last iSmash.
+    rewrite /Ψ' Nat.sub_0_r. iFrame. iIntros "!> %i %δ %Hi (HΨ & HΞ)".
+    assert (Z.to_nat (_end - beg) - δ = S $ Z.to_nat (_end - beg) - S δ) as -> by lia.
+    iSmash.
+  Qed.
+  Lemma for_spec' Ψ beg _end fn :
+    (beg ≤ _end)%Z →
+    {{{
+      ▷ Ψ beg 0 ∗
+      ( [∗ list] δ ∈ seq 0 (Z.to_nat (_end - beg)),
+        ∀ i,
+        ⌜i = (beg + δ)%Z⌝ -∗
+        Ψ i δ -∗
+        WP fn #i {{ res,
+          ⌜res = #()⌝ ∗
+          ▷ Ψ (1 + i)%Z (S δ)
+        }}
+      )
+    }}}
+      for_ #beg #_end fn
+    {{{
+      RET #();
+      Ψ _end (Z.to_nat (_end - beg))
+    }}}.
+  Proof.
+    iIntros "% %Φ H HΦ".
+    wp_apply (for_spec_strong' Ψ with "H").
+    rewrite Z.max_r //.
+  Qed.
+  Lemma for_spec_disentangled Ψ beg _end fn :
+    {{{
+      □ (
+        ∀ i δ,
+        ⌜i = (beg + δ)%Z ∧ (i < _end)%Z⌝ -∗
+        WP fn #i {{ res,
+          ⌜res = #()⌝ ∗
+          ▷ Ψ i δ
+        }}
+      )
+    }}}
+      for_ #beg #_end fn
+    {{{
+      RET #();
+      ( [∗ list] δ ∈ seq 0 (Z.to_nat (_end - beg)),
+        Ψ (beg + δ)%Z δ
+      )
+    }}}.
+  Proof.
+    iIntros "%Φ #Hfn HΦ".
+    pose (Ψ' (i : Z) δ := (
+      [∗ list] δ' ∈ seq 0 δ, Ψ (beg + δ')%Z δ'
+    )%I).
+    wp_apply (for_spec_strong Ψ'); last iSmash. iSplit; first iSmash. iIntros "!> %i %δ (%Hi1 & %Hi2) HΨ'".
+    wp_apply (wp_wand with "(Hfn [//])"). iIntros "%res (-> & HΨ)". iStep.
+    rewrite /Ψ' seq_S big_sepL_snoc. iSmash.
+  Qed.
+  Lemma for_spec_disentangled' Ψ beg _end fn :
+    {{{
+      ( [∗ list] δ ∈ seq 0 (Z.to_nat (_end - beg)),
+        ∀ i,
+        ⌜i = (beg + δ)%Z⌝ -∗
+        WP fn #i {{ res,
+          ⌜res = #()⌝ ∗
+          ▷ Ψ i δ
+        }}
+      )
+    }}}
+      for_ #beg #_end fn
+    {{{
+      RET #();
+      ( [∗ list] δ ∈ seq 0 (Z.to_nat (_end - beg)),
+        Ψ (beg + δ)%Z δ
+      )
+    }}}.
+  Proof.
+    iIntros "%Φ Hfn HΦ".
+    pose (Ψ' (i : Z) δ := (
+      [∗ list] δ' ∈ seq 0 δ, Ψ (beg + δ')%Z δ'
+    )%I).
+    wp_apply (for_spec_strong' Ψ' with "[Hfn]"); last iSmash. iSplit; first iSmash.
+    iApply (big_sepL_impl with "Hfn"). iIntros "!>" (δ δ_ (-> & Hδ)%lookup_seq) "Hfn %i -> HΨ' /=".
+    wp_apply (wp_wand with "(Hfn [//])"). iIntros "%res (-> & HΨ)". iStep.
+    rewrite /Ψ' seq_S big_sepL_snoc. iSmash.
+  Qed.
+
+  Lemma for_spec_nat_strong Ψ beg _end fn :
+    {{{
+      ▷ Ψ beg 0 ∗
+      □ (
+        ∀ i δ,
+        ⌜i = (beg + δ)%nat ∧ i < _end⌝ -∗
+        Ψ i δ -∗
+        WP fn #i {{ res,
+          ⌜res = #()⌝ ∗
+          ▷ Ψ (S i) (S δ)
+        }}
+      )
+    }}}
+      for_ #beg #_end fn
+    {{{
+      RET #();
+      Ψ (beg `max` _end) (_end - beg)
+    }}}.
+  Proof.
+    iIntros "%Φ (HΨ & #Hfn) HΦ".
+    pose Ψ' i δ :=
+      Ψ (Z.to_nat i) δ.
+    wp_apply (for_spec_strong Ψ' with "[HΨ]").
+    - rewrite /Ψ' !Nat2Z.id. iFrame. iIntros "!> %i %δ (-> & %Hδ) HΨ".
+      rewrite -Nat2Z.inj_add Z.add_1_l -Nat2Z.inj_succ !Nat2Z.id. iSmash.
+    - rewrite /Ψ' -Nat2Z.inj_max Z2Nat.inj_sub; last lia. rewrite !Nat2Z.id //.
+  Qed.
+  Lemma for_spec_nat Ψ beg _end fn :
+    beg ≤ _end →
+    {{{
+      ▷ Ψ beg 0 ∗
+      □ (
+        ∀ i δ,
+        ⌜i = (beg + δ)%nat ∧ i < _end⌝ -∗
+        Ψ i δ -∗
+        WP fn #i {{ res,
+          ⌜res = #()⌝ ∗
+          ▷ Ψ (S i) (S δ)
+        }}
+      )
+    }}}
+      for_ #beg #_end fn
+    {{{
+      RET #();
+      Ψ _end (_end - beg)
+    }}}.
+  Proof.
+    iIntros "% %Φ H HΦ".
+    wp_apply (for_spec_nat_strong Ψ with "H").
+    rewrite Nat.max_r //.
+  Qed.
+  Lemma for_spec_nat_strong' Ψ beg _end fn :
+    {{{
+      ▷ Ψ beg 0 ∗
+      ( [∗ list] δ ∈ seq 0 (_end - beg),
+        ∀ i,
+        ⌜i = (beg + δ)%nat⌝ -∗
+        Ψ i δ -∗
+        WP fn #i {{ res,
+          ⌜res = #()⌝ ∗
+          ▷ Ψ (S i) (S δ)
+        }}
+      )
+    }}}
+      for_ #beg #_end fn
+    {{{
+      RET #();
+      Ψ (beg `max` _end) (_end - beg)
+    }}}.
+  Proof.
+    iIntros "%Φ (HΨ & Hfn) HΦ".
+    pose Ψ' i δ :=
+      Ψ (Z.to_nat i) δ.
+    wp_apply (for_spec_strong' Ψ' with "[HΨ Hfn]").
+    - rewrite /Ψ' !Nat2Z.id Z2Nat.inj_sub; last lia. rewrite !Nat2Z.id. iFrame.
+      iApply (big_sepL_impl with "Hfn"). iIntros "!>" (δ δ_ (-> & Hδ)%lookup_seq) "Hfn %i -> HΨ /=".
+      rewrite -Nat2Z.inj_add Nat2Z.id Z.add_1_l -Nat2Z.inj_succ Nat2Z.id. iSmash.
+    - rewrite /Ψ' -Nat2Z.inj_max Z2Nat.inj_sub; last lia. rewrite !Nat2Z.id //.
+  Qed.
+  Lemma for_spec_nat' Ψ beg _end fn :
+    beg ≤ _end →
+    {{{
+      ▷ Ψ beg 0 ∗
+      ( [∗ list] δ ∈ seq 0 (_end - beg),
+        ∀ i,
+        ⌜i = (beg + δ)%nat⌝ -∗
+        Ψ i δ -∗
+        WP fn #i {{ res,
+          ⌜res = #()⌝ ∗
+          ▷ Ψ (S i) (S δ)
+        }}
+      )
+    }}}
+      for_ #beg #_end fn
+    {{{
+      RET #();
+      Ψ _end (_end - beg)
+    }}}.
+  Proof.
+    iIntros "% %Φ H HΦ".
+    wp_apply (for_spec_nat_strong' Ψ with "H").
+    rewrite Nat.max_r //.
+  Qed.
+  Lemma for_spec_disentangled_nat Ψ beg _end fn :
+    {{{
+      □ (
+        ∀ i δ,
+        ⌜i = (beg + δ)%nat ∧ i < _end⌝ -∗
+        WP fn #i {{ res,
+          ⌜res = #()⌝ ∗
+          ▷ Ψ i δ
+        }}
+      )
+    }}}
+      for_ #beg #_end fn
+    {{{
+      RET #();
+      ( [∗ list] δ ∈ seq 0 (_end - beg),
+        Ψ (beg + δ) δ
+      )
+    }}}.
+  Proof.
+    iIntros "%Φ #Hfn HΦ".
+    pose Ψ' i δ :=
+      Ψ (Z.to_nat i) δ.
+    wp_apply (for_spec_disentangled Ψ').
+    - iIntros "!> %i %δ (-> & %Hδ)".
+      rewrite -Nat2Z.inj_add /Ψ' Nat2Z.id. iSmash.
+    - rewrite /Ψ' Z2Nat.inj_sub; last lia. rewrite !Nat2Z.id.
+      setoid_rewrite <- Nat2Z.inj_add. setoid_rewrite Nat2Z.id.
+      iSmash.
+  Qed.
+  Lemma for_spec_disentangled_nat' Ψ beg _end fn :
+    {{{
+      ( [∗ list] δ ∈ seq 0 (_end - beg),
+        ∀ i,
+        ⌜i = (beg + δ)%nat⌝ -∗
+        WP fn #i {{ res,
+          ⌜res = #()⌝ ∗
+          ▷ Ψ i δ
+        }}
+      )
+    }}}
+      for_ #beg #_end fn
+    {{{
+      RET #();
+      ( [∗ list] δ ∈ seq 0 (_end - beg),
+        Ψ (beg + δ) δ
+      )
+    }}}.
+  Proof.
+    iIntros "%Φ Hfn HΦ".
+    pose Ψ' i δ :=
+      Ψ (Z.to_nat i) δ.
+    wp_apply (for_spec_disentangled' Ψ' with "[Hfn]").
+    - rewrite Z2Nat.inj_sub; last lia. rewrite !Nat2Z.id.
+      iApply (big_sepL_impl with "Hfn"). iIntros "!>" (δ δ_ (-> & Hδ)%lookup_seq) "Hfn %i -> /=".
+      rewrite -Nat2Z.inj_add /Ψ' Nat2Z.id. iSmash.
+    - rewrite /Ψ' Z2Nat.inj_sub; last lia. rewrite !Nat2Z.id.
+      setoid_rewrite <- Nat2Z.inj_add. setoid_rewrite Nat2Z.id.
+      iSmash.
+  Qed.
+
+  Lemma for_type τ `{!iType (iProp Σ) τ} beg _end fn :
+    {{{
+      (int_range_type beg _end --> unit_type)%T fn
+    }}}
+      for_ #beg #_end fn
+    {{{
+      RET #(); True
+    }}}.
+  Proof.
+    iIntros "%Φ #Hfn HΦ".
+    wp_apply (for_spec_disentangled (λ _ _, True%I)); iSmash.
+  Qed.
+End heap_GS.
+
+Notation "'for:' i = beg 'to' _end 'begin' e 'end'" :=
+  (for_ beg _end (λ: i, e))%E
+( i at level 1,
+  beg, _end, e at level 200,
+  format "'[hv' for:  i  =  beg  to  _end  begin  '/  ' '[' e ']'  '/' end ']'"
+) : expr_scope.
+
+#[global] Opaque for_.
